proof concept
gap buffer in c works fine

no grow yet , just made gap buffer so large

other things it needs are the view on to buffer

determine where line endings are

what does previous line mean in word wrap mode

get the view working ,
switch between word wrap and non word wrap

maybe start programming emacs , to see what is possible
maybe start programming neovim , to see what is possible

c-editor/main.c
@@ -1,0 +1,240 @@
+
+/*
+
+  
+
+a fixed sized text editor - ascii only
+
+ncurses recap
+
+initscr();      // Initialize
+endwin();       // Restore terminal
+printw(...);    // Print text
+mvprintw(y,x,); // Print at (y,x)
+refresh();      // Update screen
+clear();        // Clear screen
+getch();        // Read one key
+noecho();       // Don't echo typed keys
+cbreak();       // Disable line buffering
+keypad(stdscr, TRUE); // Enable arrow/function keys
+
+curs_set(0);   // Hide cursor
+curs_set(1);   // Normal cursor
+curs_set(2);   // Very visible cursor (if supported)
+mvaddch(y, x, ch);
+
+*/
+
+#include <stdio.h>
+#include <stdlib.h>
+#include <ncurses.h>
+
+#define BUFFER_SIZE   1000000
+#define LAST_CHAR    (BUFFER_SIZE - 1)
+
+static int buffer[BUFFER_SIZE];
+static int gap_left = 0;
+static int gap_right = BUFFER_SIZE - 1;
+
+static void clear_buffer();
+static void insert_char(int ch);
+static void delete_char();
+static void move_left();
+static void move_right();
+static void get_contents();
+
+static void clear_buffer(){
+  int i = 0;
+  for(i=0 ; i< BUFFER_SIZE ; i++){
+    buffer[i] = 0;
+  }
+}
+
+static void insert_char(int ch){
+  if (gap_left < gap_right){
+    buffer[gap_left] = ch;
+    gap_left ++;
+  }
+}
+static void delete_char(){
+  if (gap_left > 0){
+    gap_left --;
+    buffer[gap_left] = 0;    
+  }
+}
+static void move_left(){
+  if (gap_left > 0){
+    int ch = buffer[gap_left-1];
+    buffer[gap_right] = ch;
+    buffer[gap_left-1] = 0;    
+    gap_left --;
+    gap_right--;
+  }
+}
+
+static void move_right(){
+  if (gap_right >= (BUFFER_SIZE - 1)){
+    return;
+  }
+  buffer[gap_left] = buffer[gap_right+1];
+  buffer[gap_right+1] = 0;
+  gap_left ++;
+  gap_right++;  
+}
+
+static void get_contents(){
+  // todo 
+}
+
+// mean in word wrap mode , previous line on view
+static void previous_line(){
+  
+}
+
+// mean in word wrap mode , previous line on view
+static void next_line(){
+  
+}
+
+static void page_up(){
+}
+
+static void page_down(){
+}
+
+static void begin_of_line(){
+  
+}
+static void end_of_line(){
+  
+}
+
+static void redo_display(int rows,int cols){
+  // margin left
+  int mg = 2;
+  // index into buffer
+  int i = 0;
+  // tracks position on screen y x 
+  int x = 0 , y = 0;
+  // cursor x y
+  int cx = 0 , cy = 0 ,cch = 0; 
+  int ch ;
+  x = mg;
+  while(i < gap_left){
+    ch = buffer[i];
+    if (ch != '\n'){
+      mvaddch(y,x,ch);
+      if (i == (gap_left - 1)){
+	cch = ch;
+      }
+      x++;
+    }
+    else {
+      y++;
+      x=mg;
+    }
+    i ++;
+  }
+  cx = x;
+  cy = y;
+  
+  i = gap_right+1;
+  while(i <= (BUFFER_SIZE-2)){
+    ch = buffer[i];
+    if (ch != '\n'){
+      mvaddch(y,x,ch);
+      if (i == (gap_left - 1)){
+	cch = ch;
+      }
+      x++;
+    }
+    else {
+      y++;
+      x=mg;
+    }
+    i ++;
+  }
+
+  // move cursor blinky to row y , col x
+  move(cy,cx);
+  // place char on top?
+  //mvaddch(cy,cx,cch);
+    
+  
+}
+
+
+
+int main(int argc,char **argv){
+  clear_buffer();
+  initscr();
+  // Start ncurses
+  cbreak();
+  noecho();
+  keypad(stdscr,TRUE);
+  clear();
+  curs_set(1);
+  curs_set(2);
+  
+  //printw("Ready>");
+  refresh();
+  // Draw to the screen
+  // how big is the terminal ? width height
+  //
+  int ch;
+  while ((ch = getch()) != 'q') {
+    clear();
+    switch (ch) {
+    case KEY_DC:
+      // 
+      break;
+    case KEY_BACKSPACE:
+      delete_char();
+      break;
+    case KEY_IC:
+      // insert key
+      break;
+    case KEY_HOME:
+      // start of line
+      break;
+    case KEY_END:
+      // end of line
+      break;            
+    case KEY_NPAGE:
+      // page down
+      break;
+    case KEY_PPAGE:
+      // page up
+      break;      
+    case KEY_UP:
+      // move cursor a line up ??
+      break;
+    case KEY_DOWN:
+      // move cursor a line down ??
+      break;
+    case KEY_LEFT:
+      // move cursor left - remember break
+      move_left();
+      break;
+
+    case KEY_RIGHT:
+      // move cursor right - remember break
+      move_right();
+      break;
+
+    default:
+      // insert character ch - remember brek
+      insert_char(ch);
+      break;
+    }
+
+    int rows, cols;
+    getmaxyx(stdscr, rows, cols);
+    redo_display(rows,cols);
+    refresh();
+  }
+  endwin();
+  // Restore terminal
+  return 0;
+}
+
