c-editor/README.md
@@ -1,0 +1,26 @@
+# Gap Buffer
+
+gap buffer in c - for a fixed size is done in one sitting plain c 
+
+its all the other stuff around the gap buffer 
+
+window io , graphics , what want editor to do.
+
+
+difficulty want gap to grow 
+
+want view to be dynamic on resize 
+
+need to determine line , columns cursor is at 
+
+previous line in word wrap mode in the view , is not just the previous line 
+
+similarly for next line , page up , page down , 
+begin line 
+end line 
+
+how does all this fit into multiple views where do not know where the window box will be on the screen 
+oh me oh my
+
+syntax highlighting 
+
